rocq/ZF/Meta/SyntaxP.v
@@ -1,0 +1,11 @@
+Require Import ZF.Meta.Name.
+Require Import ZF.Meta.SyntaxT.
+
+Inductive Proof : Type :=
+(* An incomplete proof reference for a proposition.                             *)
+| HoleP  : Term    -> Proof
+(* An axiomatic proof reference for a proposition.                              *)
+| AxiomP : Term    -> Proof
+(* A named proof declaration applied to all its ordinary arguments.             *)
+| IdentP : Name    -> Terms -> Proof
+.
